Simplify Beta translation relation and add decision procedure

src/PlutusIR/Transform/Beta.v
@@ -1,13 +1,17 @@
-From PlutusCert Require Import
-  PlutusIR
-  Util
-  Compat
-  .
-
 From Coq Require Import
   Lists.List
   Strings.String.
 Import ListNotations.
+From PlutusCert Require Import
+  PlutusIR
+  Util
+  Compat
+  LetMergeNR
+  FreeVars
+  Util.List
+  Size
+.
+
 
 (*
 
@@ -16,80 +20,293 @@ pass has more opportunities for inlining.
 
 Transforms repeated applications (not just repeated β-redexes), e.g.
 
-         $₃
-       /  \
-     $₂    t₃
-   /  \
-  $₁   t₂
-/  \                    =>      let nonrec x = t₁
-λx t₁                                      y = t₂
-|                                          z = t₃
-λy                              in t_body
-|
-λz
-|
-t_body
+(\x y z. t) t₁ t₂ t₃
+
+=>
+
+let nonrec x = t₁
+           y = t₂
+           z = t₃
+in t
 
 *)
 
-Inductive lams : term -> list term -> list binding -> term -> Prop :=
 
-  | Lams_1 : forall t vdecls v ty t_inner arg args,
-      lams              t          args                                         vdecls  t_inner ->
-      lams (LamAbs v ty t) (arg :: args) (TermBind Strict (VarDecl v ty) arg :: vdecls) t_inner
 
-  | Lams_2 : forall t args,
-  (* ~ (exists v ty t', t = LamAbs v ty t') -> *) (* enforces the longest sequence of lambda binders *)
-      lams t args [] t
+
+Definition app_ctx := list term.
+
+Function apps (t : term) (C : app_ctx) : term :=
+  match C with
+  | [] => t
+  | s :: ss => apps (Apply t s) ss
+  end.
+
+Inductive betas : app_ctx -> term -> term -> Prop :=
+  | beta_Compat s t :
+     Compat (betas []) s t ->
+     betas [] s t
+
+  | beta_Apply C s t r :
+     betas (t :: C) s           r ->
+     betas C        (Apply s t) r
+
+  | beta_LamAbs C x T t t' t0 t0' :
+     betas C t t' ->
+     betas [] t0 t0' ->
+     (Forall (fun t => x ∉ Term.fv t) C) ->
+     betas (t0 :: C)
+      (LamAbs x T t)
+      (Let NonRec [TermBind Strict (VarDecl x T) t0'] t')
+
+  | beta_TyInst_TyAbs X K t T t' :
+      betas [] t t' ->
+      betas []
+        (TyInst (TyAbs X K t) T)
+        (Let NonRec [TypeBind (TyVarDecl X K) T] t')
+
+
+  .
+
+Lemma beta_refl : forall x, betas [] x x.
+Proof.
+  apply term__ind with (Q := fun b => Compat_Binding (betas []) b b).
+  all: try auto using betas, Compat, Compat_Bindings, Compat_Binding.
+  - intros.
+    constructor.
+    constructor.
+    + induction bs.
+      * auto using Compat_Bindings.
+      * inversion H; auto using Compat_Bindings, Compat.
+    + assumption.
+  - admit. (* TODO add Constr to Compat *)
+  - admit. (* TODO add Case to Compat *)
+Admitted.
+
+Definition spec s t := betas [] (split s) (split t).
+
+
+Require Import
+  Bool.Bool.
+From PlutusCert Require Import
+  Equality.
+
+Inductive result (A : Set) :=
+  | success
+  | failure : A -> result A
+.
+Arguments success {_}.
+Arguments failure {_} _.
+
+
+Section DEC.
+
+Context
+  (dec : list (term * (term -> bool)) -> term -> term -> bool)
+  (C : list (term * (term -> bool)))
+  (t t' : term)
 .
 
-(* accumulating param *)
-Inductive betas  : term -> list term -> list binding -> term -> Prop :=
+Definition dec_compat : bool :=
+  match C, t, t' with
+  | [], t, t' => Compat.dec_compat (dec []) t t'
+  | _, _, _ => false
+  end
+  .
 
-  | Betas_1 : forall s t args bs t_inner,
-      betas        s    (t :: args) bs t_inner ->
-      betas (Apply s t)       args  bs t_inner
+Definition dec_Apply : bool :=
+  match C, t, t' with
+  | C, Apply s t, r => dec ((t, dec [] t) :: C) s r
+  | _, _, _ => false
+  end
+.
 
-  | Betas_2 : forall t args bs t_inner,
-  (* ~ (exists t_f t_x, t = Apply t_f t_x) -> *) (* enforces the longest sequence of arguments *)
-      lams t args bs t_inner ->
-      betas t args bs t_inner
+Definition dec_TyAbs_TyInst : bool :=
+  match C, t, t' with
+  | []
+  , TyInst (TyAbs X K t) T
+  , Let NonRec [TypeBind (TyVarDecl X' K') T'] t'
+  =>
+      String.eqb X X' &&
+      Kind_eqb K K' &&
+      Ty_eqb T T' &&
+      dec [] t t'
+  | _, _, _ => false
+  end.
+
+Definition dec_LamAbs : bool :=
+  match C, t, t' with
+  | (t0, dec_t0) :: C
+  , LamAbs x T t
+  , Let NonRec [TermBind Strict (VarDecl x' T') t0'] t'
+  =>
+      String.eqb x x' &&
+      Ty_eqb T T' &&
+      dec_t0 t0' &&
+      dec C t t' &&
+      forallb (fun '(t, f) => negb (in_str x (Term.fv t))) C
+  | _, _, _ => false
+  end
+.
+
+End DEC.
+
+Fixpoint dec (C : list (term * (term -> bool))) (t t' : term) : bool :=
+     dec_compat dec C t t'
+  || dec_Apply dec C t t'
+  || dec_LamAbs dec C t t'
+  || dec_TyAbs_TyInst dec C t t'
 .
 
 
-Goal forall v1 v2 τ1 τ2 t t1 t2,
-  betas
-    (Apply (Apply (LamAbs v1 τ1 (LamAbs v2 τ2 t)) t1) t2) []
-    [TermBind Strict (VarDecl v1 τ1) t1; TermBind Strict (VarDecl v2 τ2) t2] t.
-intros.
-repeat apply Betas_1.
-apply Betas_2.
-repeat apply Lams_1.
-apply Lams_2.
+(* Defines when an argument in the (extended) application context has a
+   sound decision procedure
+*)
+Definition arg_sound '(t, dec_t) :=
+  forall t', dec_t t' = true -> betas [] t t'.
+
+Lemma dec_sound C s t :
+  Forall arg_sound C ->
+  dec C s t = true ->
+  betas (map fst C) s t.
+Proof.
+  intros H_C H_dec.
+  induction s.
+  - admit.
+  - destruct t.
+    + simpl in H_dec.
+      apply orb_prop in H_dec.
+      destruct H_dec.
+      * unfold dec_LamAbs in H.
+        destruct C. inversion H.
+        destruct p; inversion H.
+      * admit.
+    + (* Var, Var case compatibility *)
+      simpl in H_dec.
+      repeat rewrite orb_true_iff in H_dec.
+      repeat destruct H_dec as [H_dec | ?].
+      * unfold dec_compat in H_dec; destruct C.
+        ** unfold Compat.dec_compat in H_dec.
+           rewrite string_eqb_eq in H_dec.
+           subst n0.
+           constructor.
+           constructor.
+        ** inversion H_dec.
+      * inversion H.
+      * unfold dec_LamAbs in H; simpl. destruct C; inversion H; destruct p;
+      inversion H.
+      * admit.
+    + simpl in H_dec.
+  (* Needs stronger IH for terms inside Let *)
+  (* Perhaps there is a simpler IH possible that follows the function structure
+     of dec
+  *)
+Abort.
+
+Module Example.
+
+
+Open Scope string.
+
+Definition ty_unit := (Ty_Builtin DefaultUniUnit).
+Definition lam x t := LamAbs x ty_unit t.
+Definition unit := (Constant (ValueOf DefaultUniUnit tt)).
+
+Definition s :=
+  Apply
+    (Apply
+      (lam "x"
+        (lam "y" (Var "x"))
+      )
+      unit
+    )
+    unit
+.
+
+Definition s' :=
+  Let NonRec
+    [ TermBind Strict (VarDecl "x" ty_unit) unit;
+      TermBind Strict (VarDecl "y" ty_unit) unit
+    ]
+    (Var "x")
+.
+
+
+Goal betas [] (split s) (split s').
+  simpl.
+  apply beta_Apply.
+  apply beta_Apply.
+  apply beta_LamAbs.
+  apply beta_LamAbs;
+  repeat constructor. (* Why does auto using betas, Compat not work? *)
+  repeat constructor.
+  constructor.
+  simpl. intro. assumption.
+  constructor.
 Qed.
 
-Inductive beta : term -> term -> Prop :=
+Goal dec [] (split s) (split s') = true.
+Proof.
+  reflexivity.
+Qed.
 
-  | beta_multi : forall t bs bs' t_inner t_inner',
-      betas t [] bs t_inner ->
-      Compat_Bindings beta bs bs' ->
-      beta t_inner t_inner' ->
-      beta t (mk_let NonRec bs t_inner')
 
-  | beta_TyInst_TyAbs : forall ty v k t_body,
-      beta
-        (TyInst (TyAbs v k t_body) ty)
-        (Let NonRec [TypeBind (TyVarDecl v k) ty] t_body)
-
-  | beta_Compat : forall t1 t2,
-      Compat beta t1 t2 ->
-      beta t1 t2
+Definition u :=
+  (TyInst
+    (TyAbs "X" Kind_Base unit)
+    ty_unit
+  )
 .
 
+Definition v :=
+  (Let NonRec
+    [TypeBind (TyVarDecl "X" Kind_Base) ty_unit]
+    unit
+  )
+.
 
-Definition is_beta : term -> term -> bool.
-Admitted.
+Goal betas [] u v.
+  apply beta_TyInst_TyAbs.
+  repeat constructor. (* Why does auto using betas, Compat not work? *)
+Qed.
 
-Lemma is_beta_sound : forall t₁ t₂,
-  is_beta t₁ t₂ = true -> beta t₁ t₂.
-Admitted.
+Goal dec [] u v = true.
+simpl.
+reflexivity.
+Qed.
+
+(* Multi type lets is not allowed *)
+Definition w :=
+  (Apply
+    (TyInst
+      (TyAbs "X" Kind_Base
+        (LamAbs "y" (Ty_Var "X") (Var "y"))
+      )
+      ty_unit
+    )
+    unit
+  )
+.
+
+Definition x :=
+  (Let NonRec
+    [TypeBind (TyVarDecl "X" Kind_Base) ty_unit]
+    (Let NonRec
+      [TermBind Strict (VarDecl "y" (Ty_Var "X")) unit]
+      (Var "y")
+    )
+  )
+.
+
+Goal betas [] w x.
+  unfold w, x.
+  constructor.
+  Fail constructor.
+Abort.
+
+Goal dec [] w x = false.
+reflexivity.
+Qed.
+
+
+End Example.
