src/PlutusIR/Transform/LetMergeNR.v
@@ -1,6 +1,7 @@
 From PlutusCert Require Import
   PlutusIR.
 Require Import Lists.List.
+Import ListNotations.
 
 (*
 
@@ -46,9 +47,44 @@ Function merge (t : term) : term :=
   end
 .
 
+
+(* Apply split in the term of the binding *)
+Definition split_binding (split : term -> term) (b : binding) : binding :=
+  match b with
+    | TermBind s vd t => TermBind s vd (split t)
+    | DatatypeBind dtd => DatatypeBind dtd
+    | TypeBind tvd ty => TypeBind tvd ty
+  end
+  .
+
+
+(* Split non-recursive let groups into one per binding *)
+Fixpoint split (t : term) : term :=
+  match t with
+  | Let NonRec bs t =>
+      (fix go bs :=
+        match bs with
+        | [] => t
+        | b :: bs => Let NonRec [b] (go bs)
+        end) bs
+  | Let Rec bs t => Let Rec (map (split_binding split) bs) (split t)
+  | Var x => Var x
+  | TyAbs X K t => TyAbs X K (split t)
+  | LamAbs x T t => LamAbs x T (split t)
+  | Apply s t => Apply (split s) (split t)
+  | Constant c => Constant c
+  | Builtin f => Builtin f
+  | TyInst t T => TyInst (split t) T
+  | Error T => Error T
+  | IWrap F T t => IWrap F T (split t)
+  | Unwrap t => Unwrap (split t)
+  | Constr T n ts => Constr T n (map split ts)
+  | Case T t ts => Case T (split t) (map split ts)
+  end
+.
+
 Section EXAMPLES.
 
-Import ListNotations.
 Import Strings.String.
 Open Scope string_scope.
 
@@ -60,6 +96,13 @@ Definition t := Var "x".
 Example ex :
   merge (Let NonRec [b1] (Let NonRec [b2] t)) =
   Let NonRec [merge_binding merge b1; merge_binding merge b2] t.
+Proof.
+  reflexivity.
+Qed.
+
+Example split_merge :
+  split (merge (Let NonRec [b1] (Let NonRec [b2] t))) =
+  Let NonRec [b1] (Let NonRec [b2] t).
 Proof.
   reflexivity.
 Qed.
